An analysis of a function's division to two parts,
an even part and an odd part.
$$
\eqalign{
f(x) &= g(x) + h(x)\cr
g(-x) &= g(x)\cr
h(-x) &= -h(x)\cr
}
$$

Apparently, the question can be solved with linear algebra
if I can construct an equation:
$$
\left[\matrix{
1 & 1 \cr
\bigcirc & \bigcirc }\right]
\cdot
\left[\matrix{
g(x)\cr
h(x)}\right]
=
\left[\matrix{
f(x)\cr
\bigcirc}\right]
\eqno(1)
$$
The $\bigcirc$ should be replaced with something else,
and it's simple if we noticed:
$$
f(-x) = g(-x) + h(-x) = g(x) - h(x)\eqno(2)
$$
Then, we have:
$$
\left[\matrix{
1 & 1\cr
1 & -1}\right]
\cdot
\left[\matrix{
g(x)\cr
h(x)}\right]
=
\left[\matrix{
f(x)\cr
f(-x)}\right]
\eqno(3)
$$

